Require size proof for parsePngSimple

Bitmap/Basic.lean
@@ -854,40 +854,38 @@ def readChunk (bytes : ByteArray) (pos : Nat) : Option (ByteArray × ByteArray �
   else
     none
 
-def parsePngSimple (bytes : ByteArray) : Option (PngHeader × ByteArray) := do
-  if hsize : 8 <= bytes.size then
-    if bytes.extract 0 8 != pngSignature then
-      none
-    let pos := 8
-    let (typ1, data1, pos2) ← readChunk bytes pos
-    if typ1 != "IHDR".toUTF8 then
-      none
-    if hlen : data1.size ≠ 13 then
-      none
-    else
-      let hlen' : data1.size = 13 := by
-        exact not_ne_iff.mp hlen
-      let w := readU32BE data1 0 (by simp [hlen'])
-      let h := readU32BE data1 4 (by simp [hlen'])
-      let tail := data1.extract 8 13
-      if tail != ByteArray.mk #[u8 8, u8 2, u8 0, u8 0, u8 0] then
-        none
-      let hdr : PngHeader := { width := w, height := h, colorType := 2, bitDepth := 8 }
-      let (typ2, data2, pos3) ← readChunk bytes pos2
-      if typ2 != "IDAT".toUTF8 then
-        none
-      let (typ3, data3, _) ← readChunk bytes pos3
-      if typ3 != "IEND".toUTF8 then
-        none
-      if data3.size != 0 then
-        none
-      return (hdr, data2)
-  else
+def parsePngSimple (bytes : ByteArray) (_hsize : 8 <= bytes.size) :
+    Option (PngHeader × ByteArray) := do
+  if bytes.extract 0 8 != pngSignature then
     none
+  let pos := 8
+  let (typ1, data1, pos2) ← readChunk bytes pos
+  if typ1 != "IHDR".toUTF8 then
+    none
+  if hlen : data1.size ≠ 13 then
+    none
+  else
+    let hlen' : data1.size = 13 := by
+      exact not_ne_iff.mp hlen
+    let w := readU32BE data1 0 (by simp [hlen'])
+    let h := readU32BE data1 4 (by simp [hlen'])
+    let tail := data1.extract 8 13
+    if tail != ByteArray.mk #[u8 8, u8 2, u8 0, u8 0, u8 0] then
+      none
+    let hdr : PngHeader := { width := w, height := h, colorType := 2, bitDepth := 8 }
+    let (typ2, data2, pos3) ← readChunk bytes pos2
+    if typ2 != "IDAT".toUTF8 then
+      none
+    let (typ3, data3, _) ← readChunk bytes pos3
+    if typ3 != "IEND".toUTF8 then
+      none
+    if data3.size != 0 then
+      none
+    return (hdr, data2)
 
 
 partial def parsePng (bytes : ByteArray) (_hsize : 8 <= bytes.size) : Option (PngHeader × ByteArray) := do
-  if let some res := parsePngSimple bytes then
+  if let some res := parsePngSimple bytes _hsize then
     return res
   if bytes.extract 0 8 != pngSignature then
     none
